theories/rust_typing/value.v
@@ -69,8 +69,9 @@ Section value.
     assert (ot'' = ot) as -> by by eapply use_op_alg_inj.
     destruct mt; first done.
     - iPureIntro. exists ot. split_and!; [ done | | | done].
-      + destruct ot'; simpl in Hot; try destruct Hot; subst;
-          [by apply is_memcast_val_memcast.. | done ].
+      + specialize (is_memcast_val_has_layout_val' _ _ _ _ Hmc Hly) as Hly'.
+        destruct ot'; simpl in Hot; try destruct Hot; subst;
+          [apply is_memcast_val_memcast; [done | by eapply use_op_alg_wf | done].. | done ].
       + by apply has_layout_val_mem_cast.
     - iPureIntro.
       destruct ot'; simpl in Hot;
